marking certain repr args as implicits

src/3d/prelude/EverParse3D.LayeredActions.fsti
@@ -4,8 +4,8 @@ open Actions
 open Prelude
 
 let va_repr (t : Type u#a)
-            (nz:bool)
-            (k:parser_kind nz)
+            (#nz:bool)
+            (#k:parser_kind nz)
             (p:parser k t)
             (inv:slice_inv)
             (l:eloc)
@@ -14,7 +14,7 @@ let va_repr (t : Type u#a)
   = validate_with_action_t #nz #k #t p inv l allow_reading
 
 val va_return (a:Type) (x:a)
-  : va_repr a false ret_kind (parse_ret x) true_inv eloc_none true
+  : va_repr a (parse_ret x) true_inv eloc_none true
 
 val parse_bind (nz1:_) (k1:parser_kind nz1) (t1: Type u#a) (p1: parser k1 t1)
                (nz2:_) (k2:parser_kind nz2) (t2: Type u#b) (p2: (x: t1) -> parser k2 t2)
@@ -27,9 +27,9 @@ val va_bind
 //      (r1: leaf_reader p1) //<-- How to resolve this argument?
       (nz2:_) (k2:parser_kind nz2) (p2:(x:a -> parser k2 b))
       (inv2:_) (l2:_) (allow_reading2:bool)
-      (v1:va_repr a nz1 k1 p1 inv1 l1 true)
-      (v2:(x:a -> va_repr b nz2 k2 (p2 x) inv2 l2 allow_reading2))
-  : va_repr b (nz1 || nz2) (and_then_kind k1 k2)
+      (v1:va_repr a p1 inv1 l1 true)
+      (v2:(x:a -> va_repr b (p2 x) inv2 l2 allow_reading2))
+  : va_repr b
             (parse_bind _ _ _ p1 _ _ _ p2)
             (conj_inv inv1 inv2)
             (l1 `eloc_union` l2)
@@ -44,8 +44,8 @@ val subcomp (t1:Type)
             (allow_reading:bool)
             (inv2:_)
             (l2:_)
-            (v1:va_repr t1 nz1 k1 p1 inv1 l1 allow_reading)
-  : Pure (va_repr t1 nz1 k1 p1 inv2 l2 allow_reading)
+            (v1:va_repr t1 p1 inv1 l1 allow_reading)
+  : Pure (va_repr t1 p1 inv2 l2 allow_reading)
          (requires inv2 `inv_implies` inv1 /\
                    l2 `eloc_includes` l1)
          (ensures fun _ -> True)
@@ -57,18 +57,18 @@ let if_then_else (t1:Type)
                  (inv1:_)
                  (l1:_)
                  (allow_reading:bool)
-                 (v1:va_repr t1 nz1 k1 p1 inv1 l1 allow_reading)
-                 (v2:va_repr t1 nz1 k1 p1 inv1 l1 allow_reading)
+                 (v1:va_repr t1 p1 inv1 l1 allow_reading)
+                 (v2:va_repr t1 p1 inv1 l1 allow_reading)
                  (p:Type0)
   : Type
-  = va_repr t1 nz1 k1 p1 inv1 l1 allow_reading
+  = va_repr t1 p1 inv1 l1 allow_reading
 
 //#push-options "--debug EverParse3D.LayeredActions --debug_level LayeredEffectsTc"
 reifiable reflectable
 layered_effect {
   VA_ : t : Type
-     -> nz:bool
-     -> k:parser_kind nz
+     -> #nz:bool
+     -> #k:parser_kind nz
      -> p:parser k t
      -> inv:slice_inv
      -> l:eloc
@@ -85,20 +85,16 @@ layered_effect {
 
 // sub_effect PURE ~> RSTATE = lift_pure_rst
 
-effect VA (t:Type) (#nz:bool) (#k:parser_kind nz) (p:parser k t) (inv:slice_inv) (l:eloc) (allow_reading:bool) =
-  VA_ t nz k p inv l allow_reading
-
-
 let lift_pure (a:Type) (f:unit -> Tot a)
-  : Tot (va_repr a false ret_kind (parse_ret (f())) true_inv eloc_none true)
+  : Tot (va_repr a (parse_ret (f())) true_inv eloc_none true)
   = va_return a (f())
 
 sub_effect PURE ~> VA_ = lift_pure
 
 
-val va_ret (#a:Type) (x:a) : VA a (parse_ret x) true_inv eloc_none false
+val va_ret (#a:Type) (x:a) : VA_ a (parse_ret x) true_inv eloc_none false
 
-val va_u16 (_:unit) : VA ___UINT16 parse____UINT16 true_inv eloc_none true
+val va_u16 (_:unit) : VA_ ___UINT16 parse____UINT16 true_inv eloc_none true
 
 let parse_pair (#nz1:_) (#k1:parser_kind nz1) (#t1:_) (p1:parser k1 t1)
                (#nz2:_) (#k2:parser_kind nz2) (#t2:_) (p2:parser k2 t2)
@@ -107,7 +103,7 @@ let parse_pair (#nz1:_) (#k1:parser_kind nz1) (#t1:_) (p1:parser k1 t1)
     parse_bind _ _ _ p2 _ _ _ (fun x2 ->
     parse_ret (x1, x2)))
 
-let test (_:unit) : VA (___UINT16 * ___UINT16)
+let test (_:unit) : VA_ (___UINT16 * ___UINT16)
                        (parse_pair parse____UINT16 parse____UINT16)
                        (conj_inv true_inv (conj_inv true_inv true_inv))
                        (eloc_union eloc_none (eloc_union eloc_none eloc_none))
@@ -116,7 +112,7 @@ let test (_:unit) : VA (___UINT16 * ___UINT16)
     let x2 = va_u16 () in
     va_ret (x1, x2)
 
-let test2 (_:unit) : VA (___UINT16 * ___UINT16)
+let test2 (_:unit) : VA_ (___UINT16 * ___UINT16)
                        (parse_pair parse____UINT16 parse____UINT16)
                        true_inv
                        eloc_none
@@ -134,15 +130,15 @@ let parse_dep_pair (#nz1:_) (#k1:parser_kind nz1) (#t1:_) (p1:parser k1 t1)
 
 inline_for_extraction noextract
 val va_filter (#nz:_) (#k:parser_kind nz) (#t:_) (#p:parser k t)
-              (#inv:_) (#l:_) (v:unit -> VA t p inv l true)
+              (#inv:_) (#l:_) (v:unit -> VA_ t p inv l true)
               // (r:leaf_reader p)
     (f:t -> bool)
-  : VA_ (refine t f) nz (filter_kind k) (p `parse_filter` f) inv l false
+  : VA_ (refine t f) (p `parse_filter` f) inv l false
 
 val gt (x:int) (y:___UINT16) : bool
 
 #push-options "--print_implicits --print_universes --print_effect_args"
-let test3 (_:unit) : VA ___UINT16
+let test3 (_:unit) : VA_ ___UINT16
                        parse____UINT16
                        true_inv
                        eloc_none
